define signatures and rows as in paper version

theories/logic/sem_row.v
@@ -19,10 +19,13 @@ From affect.logic Require Import sem_def.
 From affect.logic Require Import mode.
 From affect.logic Require Import sem_sig.
 
+(* Nil Row *)
 Program Definition sem_row_nil {Σ} : sem_row Σ := @SemRow Σ ⊥ _. 
 Next Obligation. iIntros (???) "[]". Qed.
+
 Global Instance sem_row_bottom {Σ} : Bottom (sem_row Σ) := sem_row_nil.
 
+(* Cons Row *)
 Program Definition sem_row_cons {Σ} (op : operation) : sem_sig Σ -d> sem_row Σ -d> sem_row Σ :=
     λ σ ρ, (@SemRow Σ (@PMonoProt Σ (IEff 
               (λ v, λne Φ, ∃ (op' : operation) (v' : val), 
@@ -46,25 +49,21 @@ Next Obligation.
   iIntros (??????) "(%op' & %v' & -> & H)". by iExists op', v'.
 Qed.
 
-Program Definition sem_row_flip_bang {Σ} (ρ : sem_row Σ) : sem_row Σ := 
-  @SemRow Σ (@PMonoProt Σ (upcl OS ρ) _) _.
-Next Obligation.
-  iIntros (?????) "#HΦ Hσ".
-  pose proof (upcl_mono_prot ρ) as []. 
-  iApply (monotonic_prot with "HΦ Hσ").
+Global Instance sem_row_cons_ne {Σ} op : NonExpansive2 (@sem_row_cons Σ op).
+Proof. 
+  intros ???????. rewrite /sem_row_cons. 
+  intros ??. simpl. do 7 f_equiv; first f_equiv; apply non_dep_fun_dist; by f_equiv.  
 Qed.
-Next Obligation.
-  iIntros (????) "(%Φ' & Hρ & _)".
-  iApply (sem_row_prop _ ρ with "Hρ").
+Global Instance sem_row_cons_Proper {Σ} op : Proper ((≡) ==> (≡) ==> (≡)) (@sem_row_cons Σ op).
+Proof. apply ne_proper_2. apply _. Qed.
+
+Global Instance sem_row_cons_contractive {Σ} op n : Proper (dist_later n ==> dist n ==> dist n) (@sem_row_cons Σ op).
+Proof. 
+  intros ???????. rewrite /sem_row_cons. 
+  intros ?. simpl. do 6 f_equiv; first f_contractive; f_equiv; apply non_dep_fun_dist; by f_equiv.
 Qed.
 
-(* generalised flip-bang row *)
-Notation "¡_[ m ] ρ" := (
-  match m with
-      OS => sem_row_flip_bang ρ
-    | MS => ρ
-  end) (at level 10) : sem_row_scope.
-
+(* Recursive Row *)
 Definition sem_row_rec {Σ} (R : sem_row Σ → sem_row Σ) `{Contractive R} : sem_row Σ :=
   fixpoint R.
 
@@ -76,130 +75,42 @@ Lemma sem_row_rec_unfold_iEff {Σ} (R : sem_row Σ → sem_row Σ) `{Contractive
   iEff_car (sem_row_rec R) v Φ ≡ iEff_car (R (sem_row_rec R)) v Φ.
 Proof. f_equiv. apply non_dep_fun_equiv. rewrite {1}sem_row_rec_unfold //. Qed.
 
-(*  Properties *)
-
-Global Instance sem_row_cons_ne {Σ} op : NonExpansive2 (@sem_row_cons Σ op).
-Proof. 
-  intros ???????. rewrite /sem_row_cons. 
-  intros ??. simpl. do 7 f_equiv; first f_equiv; apply non_dep_fun_dist; by f_equiv.  
+(* Flip-Bang Row *)
+Program Definition sem_row_flip_mbang {Σ} (m : mode) (ρ : sem_row Σ) : sem_row Σ := 
+  @SemRow Σ (@PMonoProt Σ (upcl m ρ) _) _.
+Next Obligation.
+  iIntros (??????) "#HΦ Hσ". 
+  destruct m.
+  - pose proof (upcl_mono_prot ρ) as []. 
+    iApply (monotonic_prot with "HΦ Hσ").
+  - pose proof (pers_upcl_pers_mono_prot ρ) as [].
+    iApply (pers_monotonic_prot with "HΦ Hσ").
 Qed.
-Global Instance sem_row_cons_Proper {Σ} op : Proper ((≡) ==> (≡) ==> (≡)) (@sem_row_cons Σ op).
-Proof. apply ne_proper_2. apply _. Qed.
-Global Instance sem_row_cons_contractive {Σ} op n : Proper (dist_later n ==> dist n ==> dist n) (@sem_row_cons Σ op).
-Proof. 
-  intros ???????. rewrite /sem_row_cons. 
-  intros ?. simpl. do 6 f_equiv; first f_contractive; f_equiv; apply non_dep_fun_dist; by f_equiv.
+Next Obligation.
+  iIntros (?????) "(%Φ' & Hρ & _)".
+  iApply (sem_row_prop _ ρ with "Hρ").
 Qed.
 
-Global Instance sem_row_flip_bang_ne {Σ} : NonExpansive (@sem_row_flip_bang Σ).
-Proof. intros ?????. rewrite /sem_row_flip_bang. intros ?. simpl. 
+Global Instance sem_row_flip_mbang_ne {Σ} m : NonExpansive (@sem_row_flip_mbang Σ m).
+Proof. intros ?????. rewrite /sem_row_flip_mbang. intros ?. simpl. 
        do 4 f_equiv. apply non_dep_fun_dist; by f_equiv. Qed.
-Global Instance sem_row_flip_bang_Proper {Σ} : Proper ((≡) ==> (≡)) (@sem_row_flip_bang Σ).
+Global Instance sem_row_flip_bang_Proper {Σ} m : Proper ((≡) ==> (≡)) (@sem_row_flip_mbang Σ m).
 Proof. apply ne_proper. apply _. Qed.
 
-Global Instance sem_row_flip_bang_rec_contractive {Σ} (R : sem_row Σ -d> sem_row Σ) `{Contractive R} : 
-  Contractive (λ θ, sem_row_flip_bang (R θ)).
+Global Instance sem_row_flip_mbang_rec_contractive {Σ} m (R : sem_row Σ -d> sem_row Σ) `{Contractive R} : 
+  Contractive (λ θ, sem_row_flip_mbang m (R θ)).
 Proof.
-  intros ??????. rewrite /sem_row_flip_bang. simpl.
+  intros ??????. rewrite /sem_row_flip_mbang. simpl.
   do 4 f_equiv. apply non_dep_fun_dist. by apply Contractive0.
 Qed. 
 
 (* Notations. *)
-
 Notation "⟨⟩" := (sem_row_nil) : sem_row_scope.
 Notation "opσ · ρ" := (sem_row_cons opσ.1%S opσ.2%S ρ%R) (at level 80, right associativity) : sem_row_scope.
-Notation "¡ ρ" := (sem_row_flip_bang ρ%R) (at level 10) : sem_row_scope.
+Notation "¡_[ m ] ρ" := (sem_row_flip_mbang m ρ) (at level 10) : sem_row_scope.
 Notation "'μR:' θ , ρ " := (sem_row_rec (λ θ, ρ%R)) (at level 50) : sem_row_scope.
 
-(* One-Shot Rows *)
-
-Global Instance row_nil_once {Σ} : Once (⟨⟩ : sem_row Σ)%R.
-Proof. constructor. rewrite /= /sem_row_nil. iIntros (v Φ Φ') "_ []". Qed.
-
-Global Instance row_cons_once {Σ} (ρ : sem_row Σ) op (σ : sem_sig Σ) `{! Once σ, ! Once ρ } :
-  Once ((op, σ) · ρ).
-Proof.
-  constructor. rewrite /sem_row_cons /=. 
-  iIntros (v Φ Φ') "HPost (%op' & %v' & -> & H)".
-  destruct (decide (op = op')) as [->|].
-  - iExists op', v'; iSplit; try done. 
-    rewrite decide_True; last auto. 
-    inv H. iDestruct (monotonic_prot with "HPost") as "Hσ".
-    by iApply "Hσ".
-  - iExists op', v'; iSplit; try done. 
-    rewrite decide_False; last auto.
-    inv H0. iDestruct (monotonic_prot with "HPost") as "Hρ".
-    by iApply "Hρ".
-Qed.
-
-Global Instance row_fbang_once {Σ} (ρ : sem_row Σ) : Once (¡ ρ)%R.
-Proof.
-  constructor. rewrite /sem_row_flip_bang.
-  pose proof (upcl_mono_prot ρ) as []. iIntros (???).
-  iIntros "HPost /= H". 
-  iApply (monotonic_prot v Φ Φ' with "HPost H").
-Qed.
-
-Global Instance row_rec_once {Σ} (R : sem_row Σ → sem_row Σ) `{Contractive R} :
-  (∀ θ, Once (R θ)) → Once (μR: θ, R θ).
-Proof.
-  intros H. constructor. 
-  iIntros (???) "HPost H". rewrite !sem_row_rec_unfold_iEff.
-  specialize (H (μR: θ, R θ)%R). inv H. by iApply (monotonic_prot with "HPost").
-Qed.
-
-(* Substructurality relation on rows wrt to types and environments *)
-
-Definition mono_prot_on_prop {Σ} (Ψ : iEff Σ) (P : iProp Σ) : iProp Σ :=
-  □ (∀ v Φ, iEff_car Ψ v Φ -∗ P -∗ iEff_car Ψ v (λ w, Φ w ∗ P))%I.
-
-(* For semantic signatures, being monotonic on all propositions is the same as being monotonic
-   because semantic signatures are persistently monotonic by definition *)
-Lemma mono_prot_on_prop_monotonic {Σ} (σ : sem_sig Σ) : 
-  (⊢ ∀ P, mono_prot_on_prop σ P) ↔ MonoProt σ.
-Proof.
-  split.
-  - iIntros (H). constructor. iIntros (v Φ Φ') "Hpost HΨ".
-    iDestruct (H with "HΨ Hpost") as "H".
-    iApply (pmono_prot_prop _ σ with "[] H").
-    { iIntros "!# % [HΦ HPost]". by iApply "HPost". }
-  - iIntros (H) "%P %v %Φ !# Hσ HP". inv H.
-    iApply (monotonic_prot with "[HP] Hσ"). iIntros (?) "$ //".
-Qed.
-
-Definition row_type_sub {Σ} (ρ : sem_row Σ) (τ : sem_ty Σ) : iProp Σ := 
-  (∀ v, mono_prot_on_prop ρ (τ v)).
-
-Notation "ρ ≼ₜ τ" := (row_type_sub ρ%R τ%T)%I (at level 80) : bi_scope.
-
-Lemma row_type_sub_once {Σ} (ρ : sem_row Σ) (τ : sem_ty Σ) `{Once ρ} : ⊢ ρ ≼ₜ τ.
-Proof.
-  iIntros (w v Φ) "!# Hρ Hτ".
-  iApply (monotonic_prot v Φ (λ w', Φ w' ∗ τ w)%I with "[Hτ] Hρ").
-  iIntros "% $ //".
-Qed.
-
-Lemma row_type_sub_fbang {Σ} (ρ : sem_row Σ) (τ : sem_ty Σ) : ⊢ (¡ ρ) ≼ₜ τ.
-Proof.
-  iApply row_type_sub_once.
-Qed.
-
-Definition row_env_sub {Σ} (ρ : sem_row Σ) (Γ : env Σ) : iProp Σ := 
-  (∀ vs, mono_prot_on_prop ρ (⟦ Γ ⟧ vs)).
-
-Notation "ρ ≼ₑ Γ" := (row_env_sub ρ%R Γ%T) (at level 80) : bi_scope.
-
-Lemma row_env_sub_once {Σ} (ρ : sem_row Σ) (Γ : env Σ) `{Once ρ} : ⊢ ρ ≼ₑ Γ.
-Proof.
-  iIntros (γ v Φ) "!# Hρ HΓ".
-  iApply (monotonic_prot v Φ (λ w', Φ w' ∗ ⟦ Γ ⟧ γ)%I with "[HΓ] Hρ").
-  iIntros "% $ //".
-Qed.
-
-Lemma row_env_sub_fbang {Σ} (ρ : sem_row Σ) (Γ : env Σ) : ⊢ (¡ ρ) ≼ₑ Γ.
-Proof. iApply row_env_sub_once. Qed.
-
-(* Subsumption relation on rows *)
+(* Subtyping on Rows *)
 
 Lemma row_le_refl {Σ} (ρ : sem_row Σ) :
   ⊢ ρ ≤R ρ.
@@ -224,104 +135,6 @@ Proof.
   iExists op', v'; iSplit; first done.
   destruct (decide (op = op')); first (by iApply "Hσσ'"). 
   by iApply "Hρρ'".
-Qed.
-
-Lemma row_le_rec_unfold {Σ} (R : sem_row Σ → sem_row Σ) `{Contractive R} :
-  ⊢ (μR: θ, R θ) ≤R R (μR: θ, R θ).
-Proof. rewrite {1} sem_row_rec_unfold //. iApply row_le_refl. Qed.
-
-Lemma row_le_rec_fold {Σ} (R : sem_row Σ → sem_row Σ) `{ Contractive R }:
-  ⊢ R (μR: θ, R θ) ≤R (μR: θ, R θ).
-Proof. rewrite - {1} sem_row_rec_unfold. iApply row_le_refl. Qed.
-
-Lemma row_le_mfbang_cons {Σ} op m σ (ρ : sem_row Σ) :
-  ⊢ ¡_[ m ] ((op, σ) · ρ) ≤R (op, ¡_[ m ] σ)%S · (¡_[ m ] ρ).
-Proof. 
-  rewrite /sem_row_flip_bang. destruct m; last iApply row_le_refl.
-  iIntros (??) "!# (%Φ' & (%op' & %v' & -> & H) & Hpost)". simpl.
-  iExists op', v'. iSplit; first done.
-  destruct (decide (op = op')); first iNext; iExists Φ'; iFrame. 
-Qed.
-
-Corollary row_le_mfbang_cons_os {Σ} op m (σ : sem_sig Σ) (ρ : sem_row Σ) `{Once σ}:
-  ⊢ ¡_[ m ] ((op, σ) · ρ) ≤R (op, σ)%S · (¡_[ m ] ρ).
-Proof. 
-  iApply row_le_trans; first iApply row_le_mfbang_cons.
-  iApply row_le_cons_comp; last iApply row_le_refl.
-  iApply sig_le_mfbang_elim.
-Qed.
-
-Corollary row_le_mfbang_cons_eff {Σ} op m {TT : tele} (ι κ : tele_arg TT → sem_ty Σ) (ρ : sem_row Σ) :
-  ⊢ ¡_[ m ] ((op, ∀S..: α , ι α =[ m ]=> κ α) · ρ) ≤R (op, (∀S..: α , ι α =[ m ]=> κ α)%S) · (¡_[ m ] ρ).
-Proof. 
-  iApply row_le_trans; first iApply row_le_mfbang_cons.
-  iApply row_le_cons_comp; last iApply row_le_refl.
-  iApply sig_le_mfbang_elim_eff.
-Qed.
-
-Lemma row_le_mfbang_comp {Σ} (m : mode) (ρ ρ' : sem_row Σ) :
-  ρ ≤R ρ' -∗
-  ¡_[ m ] ρ ≤R ¡_[ m ] ρ'. 
-Proof. 
-  iIntros "#Hle". destruct m; last iApply "Hle".
-  rewrite /sem_row_flip_bang. 
-  iIntros (??) "!# (%Φ' & Hρ & Hpost)". simpl.
-  iExists Φ'. iFrame. by iApply "Hle".
-Qed.
-
-Lemma row_le_mfbang_intro {Σ} (m : mode) (ρ : sem_row Σ) :
-  ⊢ ρ ≤R ¡_[ m ] ρ. 
-Proof. 
-  destruct m; last iApply row_le_refl.
-  rewrite /sem_row_flip_bang. iIntros (??) "!# Hρ". simpl.
-  iExists Φ. iFrame. iIntros (?) "$ //".
-Qed.
-
-Lemma row_le_mfbang_elim {Σ} m (ρ : sem_row Σ) `{! Once ρ}:
-  ⊢ ¡_[m] ρ ≤R ρ. 
-Proof. 
-  destruct m; simpl; last iApply row_le_refl.
-  rewrite /sem_row_flip_bang. iIntros (??) "!# (%Φ' & Hρ & Hpost)". simpl.
-  inv H. by iApply (monotonic_prot with "Hpost").
-Qed.
-
-Lemma row_le_mfbang_comm {Σ} m m' (ρ : sem_row Σ) :
-  ⊢ ¡_[m] (¡_[m'] ρ) ≤R ¡_[m'] (¡_[m] ρ).
-Proof. 
-  destruct m, m'; iApply row_le_refl.
-Qed.
-
-Lemma row_le_mfbang_mode_le {Σ} m m' (ρ : sem_row Σ) :
-  ⊢ m' ≤M m -∗ (¡_[m] ρ) ≤R (¡_[m'] ρ).
-Proof. 
-  iIntros "H". destruct m.
-  - iDestruct (mode_le_OS_inv with "H") as "->".
-    iApply sig_le_refl.
-  - iApply row_le_mfbang_intro.
-Qed.
-
-Corollary row_le_fbang_nil {Σ} m :
-   ⊢ ¡_[m] ⟨⟩%R ≤R (⟨⟩%R : sem_row Σ).
-Proof. 
-  destruct m; simpl; last iApply row_le_refl.
-  apply (row_le_mfbang_elim OS). apply _. 
-Qed.
-
-Corollary row_le_fbang_idemp {Σ} m (ρ : sem_row Σ) :
-   ⊢ ¡_[m] (¡_[m] ρ) ≤R ¡_[m] ρ.
-Proof. 
-  destruct m; simpl; last iApply row_le_refl.
-  apply (row_le_mfbang_elim OS). apply _. 
-Qed.
-
-Corollary row_le_mfbang_rec {Σ} (m : mode) (R : sem_row Σ → sem_row Σ) `{ Contractive R }: 
-  (∀ θ, ¡_[ m ] (R θ) ≤R (R θ)) -∗ ¡_[ m ] (μR: θ, R θ) ≤R (μR: θ, R θ).
-Proof. 
-  iIntros "#Hle". destruct m; last iApply row_le_refl.
-  iApply row_le_trans.
-  { iApply (row_le_mfbang_comp OS). iApply row_le_rec_unfold. }
-  iApply row_le_trans; first iApply "Hle". 
-  iApply row_le_rec_fold.
 Qed.
 
 Lemma row_le_swap_second {Σ} (op op' : operation) (σ σ' : sem_sig Σ) (ρ : sem_row Σ) : 
@@ -363,3 +176,177 @@ Proof.
   iApply row_le_trans; first iApply row_le_cons_comp; [iApply sig_le_refl|by iApply row_le_swap_third|].
   by iApply row_le_swap_second.
 Qed.
+
+Lemma row_le_rec_unfold {Σ} (R : sem_row Σ → sem_row Σ) `{Contractive R} :
+  ⊢ (μR: θ, R θ) ≤R R (μR: θ, R θ).
+Proof. rewrite {1} sem_row_rec_unfold //. iApply row_le_refl. Qed.
+
+Lemma row_le_rec_fold {Σ} (R : sem_row Σ → sem_row Σ) `{ Contractive R }:
+  ⊢ R (μR: θ, R θ) ≤R (μR: θ, R θ).
+Proof. rewrite - {1} sem_row_rec_unfold. iApply row_le_refl. Qed.
+
+Lemma row_le_mfbang_intro {Σ} (m : mode) (ρ : sem_row Σ) :
+  ⊢ ρ ≤R ¡_[ m ] ρ. 
+Proof. 
+  rewrite /sem_row_flip_mbang. iIntros (??) "!# Hρ". simpl.
+  iExists Φ. iFrame. iApply bi.intuitionistically_intuitionistically_if. 
+  iIntros "!# % $ //".
+Qed.
+
+Lemma row_le_mfbang_elim_ms {Σ} (ρ : sem_row Σ) :
+  ⊢ ¡_[MS] ρ ≤R ρ. 
+Proof. 
+  rewrite /sem_sig_flip_mbang. 
+  iIntros (v Φ) "!# (%Φ' & Hρ & HPost)". simpl.
+  by iApply (@pmono_prot_prop Σ ρ with "HPost").
+Qed.
+
+Lemma row_le_mfbang_comp {Σ} m m' (ρ ρ' : sem_row Σ) :
+  m' ≤M m -∗ ρ ≤R ρ' -∗
+  (¡_[m] ρ) ≤R (¡_[m'] ρ').
+Proof. 
+  iIntros "#Hlem #Hleσ". destruct m.
+  - iDestruct (mode_le_OS_inv with "Hlem") as "->".
+    rewrite /row_le /sem_row_flip_mbang /tc_opaque.
+    by iApply iEff_le_upcl.
+  - iApply row_le_trans; first iApply row_le_mfbang_elim_ms. 
+    iApply row_le_trans; first iApply (row_le_mfbang_intro m').
+    rewrite /row_le /sem_row_flip_mbang /tc_opaque.
+    by iApply iEff_le_upcl.
+Qed.
+
+Lemma row_le_mfbang_cons {Σ} op m σ (ρ : sem_row Σ) :
+  ⊢ ¡_[ m ] ((op, σ) · ρ) ≤R (op, ¡_[ m ] σ)%S · (¡_[ m ] ρ).
+Proof. 
+  rewrite /sem_row_flip_mbang. 
+  iIntros (??) "!# (%Φ' & (%op' & %v' & -> & H) & Hpost)". simpl.
+  iExists op', v'. iSplit; first done.
+  destruct (decide (op = op')); first iNext; iExists Φ'; iFrame. 
+Qed.
+
+Lemma row_le_mfbang_idemp {Σ} m (ρ : sem_row Σ) :
+  ⊢ (¡_[ m ] (¡_[ m ] ρ)) ≤R ((¡_[ m ] ρ)).
+Proof. 
+  iIntros (v Φ) "!# (%Φ' & (%Φ'' & H & HPost') & HPost)". 
+  rewrite /sem_row_flip_mbang /=.
+  iDestruct (bi.intuitionistically_if_sep_2 with "[HPost HPost']") as "HP"; first iFrame.
+  iExists Φ''. iFrame.
+  iApply (bi.intuitionistically_if_mono with "HP").
+  iIntros "[H1 H2] % HΦ''". iApply ("H2" with "[H1 HΦ'']"). 
+  by iApply "H1".
+Qed.
+
+Lemma row_le_mfbang_comm {Σ} m m' (ρ : sem_row Σ) :
+  ⊢ (¡_[ m ] (¡_[ m' ] ρ)) ≤R (¡_[ m' ] (¡_[ m ] ρ)).
+Proof. 
+  destruct m, m'.
+  - iApply row_le_refl.
+  - iApply row_le_trans; first iApply row_le_mfbang_comp.
+    { iApply mode_le_refl. }
+    { iApply row_le_mfbang_elim_ms. }
+    iApply row_le_mfbang_intro.
+  - iApply row_le_trans; first iApply row_le_mfbang_elim_ms.
+    iApply row_le_mfbang_comp; first iApply mode_le_refl. iApply row_le_mfbang_intro.
+  - iApply row_le_refl.
+Qed.
+
+Lemma row_le_mfbang_nil {Σ} m :
+   ⊢ ¡_[m] ⟨⟩%R ≤R (⟨⟩%R : sem_row Σ).
+Proof. 
+  destruct m; simpl; last iApply row_le_mfbang_elim_ms.
+  iIntros (??) "!# (% & [] & _)".
+Qed.
+
+Lemma row_le_mfbang_rec {Σ} (m : mode) (R : sem_row Σ → sem_row Σ) `{ Contractive R }: 
+  (∀ θ, ¡_[ m ] (R θ) ≤R (R θ)) -∗ ¡_[ m ] (μR: θ, R θ) ≤R (μR: θ, R θ).
+Proof. 
+  iIntros "#Hle". destruct m; last iApply row_le_mfbang_elim_ms.
+  iIntros (??) "!# (%Φ' & H & HP)". simpl.
+  iApply sem_row_rec_unfold_iEff. rewrite sem_row_rec_unfold_iEff.
+  iApply "Hle". iExists Φ'. simpl. iFrame.
+Qed.
+
+(* Once Constraint *)
+
+Class OnceR {Σ} (ρ : sem_row Σ) := {
+  flip_mbang_elim : (⊢ (¡_[ OS ] ρ%R) ≤R ρ%R)
+}.
+
+Global Instance row_nil_once {Σ} : OnceR (⟨⟩ : sem_row Σ)%R.
+Proof. constructor. iApply row_le_mfbang_nil. Qed.
+
+Global Instance row_cons_once {Σ} (ρ : sem_row Σ) op (σ : sem_sig Σ) `{! OnceS σ, ! OnceR ρ } :
+  OnceR ((op, σ) · ρ)%R.
+Proof.
+  constructor. inv OnceS0. inv OnceR0.
+  iApply row_le_trans; first iApply row_le_mfbang_cons.
+  iApply row_le_cons_comp; [iApply flip_mbang_elim0|iApply flip_mbang_elim1].
+Qed.
+
+Global Instance row_fbang_once {Σ} (ρ : sem_row Σ) : OnceR (¡_[OS] ρ)%R.
+Proof. constructor. iApply row_le_mfbang_idemp. Qed.
+
+Global Instance row_rec_once {Σ} (R : sem_row Σ → sem_row Σ) `{Contractive R} :
+  (∀ θ, OnceR (R θ)) → OnceR (μR: θ, R θ)%R.
+Proof.
+  intros H. constructor. 
+  iApply row_le_mfbang_rec. iIntros (θ). 
+  destruct (H θ). iApply flip_mbang_elim0.
+Qed.
+
+Global Instance monoprot_once {Σ} (ρ : sem_row Σ) `{! OnceR ρ } : MonoProt ρ.
+Proof.
+  constructor. iIntros (???) "HP Hρ".
+  inv OnceR0. iApply flip_mbang_elim0.
+  iExists Φ. simpl. iFrame.
+Qed.
+
+(* Substructurality relation on rows wrt to types and environments *)
+
+Definition mono_prot_on_prop {Σ} (Ψ : iEff Σ) (P : iProp Σ) : iProp Σ :=
+  □ (∀ v Φ, iEff_car Ψ v Φ -∗ P -∗ iEff_car Ψ v (λ w, Φ w ∗ P))%I.
+
+(* For semantic signatures, being monotonic on all propositions is the same as being monotonic
+   because semantic signatures are persistently monotonic by definition *)
+Lemma mono_prot_on_prop_monotonic {Σ} (σ : sem_sig Σ) : 
+  (⊢ ∀ P, mono_prot_on_prop σ P) ↔ MonoProt σ.
+Proof.
+  split.
+  - iIntros (H). constructor. iIntros (v Φ Φ') "Hpost HΨ".
+    iDestruct (H with "HΨ Hpost") as "H".
+    iApply (pmono_prot_prop _ σ with "[] H").
+    { iIntros "!# % [HΦ HPost]". by iApply "HPost". }
+  - iIntros (H) "%P %v %Φ !# Hσ HP". inv H.
+    iApply (monotonic_prot with "[HP] Hσ"). iIntros (?) "$ //".
+Qed.
+
+Definition row_type_sub {Σ} (ρ : sem_row Σ) (τ : sem_ty Σ) : iProp Σ := 
+  (∀ v, mono_prot_on_prop ρ (τ v)).
+
+Notation "ρ ≼ₜ τ" := (row_type_sub ρ%R τ%T)%I (at level 80) : bi_scope.
+
+Lemma row_type_sub_once {Σ} (ρ : sem_row Σ) (τ : sem_ty Σ) `{! OnceR ρ} : ⊢ ρ ≼ₜ τ.
+Proof.
+  iIntros (w v Φ) "!# Hρ Hτ". 
+  iApply (monotonic_prot v Φ (λ w', Φ w' ∗ τ w)%I with "[Hτ] Hρ").
+  iIntros "% $ //".
+Qed.
+
+Lemma row_type_sub_fbang {Σ} (ρ : sem_row Σ) (τ : sem_ty Σ) : ⊢ (¡_[OS] ρ) ≼ₜ τ.
+Proof. iApply row_type_sub_once. Qed.
+
+Definition row_env_sub {Σ} (ρ : sem_row Σ) (Γ : env Σ) : iProp Σ := 
+  (∀ vs, mono_prot_on_prop ρ (⟦ Γ ⟧ vs)).
+
+Notation "ρ ≼ₑ Γ" := (row_env_sub ρ%R Γ%T) (at level 80) : bi_scope.
+
+Lemma row_env_sub_once {Σ} (ρ : sem_row Σ) (Γ : env Σ) `{! OnceR ρ} : ⊢ ρ ≼ₑ Γ.
+Proof.
+  iIntros (γ v Φ) "!# Hρ HΓ".
+  iApply (monotonic_prot v Φ (λ w', Φ w' ∗ ⟦ Γ ⟧ γ)%I with "[HΓ] Hρ").
+  iIntros "% $ //".
+Qed.
+
+Lemma row_env_sub_fbang {Σ} (ρ : sem_row Σ) (Γ : env Σ) : ⊢ (¡_[OS] ρ) ≼ₑ Γ.
+Proof. iApply row_env_sub_once. Qed.
+
